theories/tests/add.v
@@ -10,7 +10,7 @@ Section example.
   Context `{clangG Σ, refineG Σ} {N: namespace}.
 
   Parameter py: addr.
-  Definition I := (∃ vy, py ↦ Vint32 vy @ Tint32 ∗ own_sstate {[ "Y" := Vint32 vy ]})%I.
+  Definition I := (∃ vy, py ↦ Vint8 vy @ Tint8 ∗ own_sstate {[ "Y" := Vint8 vy ]})%I.
 
   Definition invs (prio: nat) : iProp Σ :=
     match prio with
@@ -22,28 +22,28 @@ Section example.
 
   Definition f_body : expr :=
     cli i ;;
-    py <- !py@Tint32 + "x" ;;
-    "x" <- !py@Tint32 ;;
+    py <- !py@Tint8 + "x" ;;
+    "x" <- !py@Tint8 ;;
     sti i ;;
     return: "x".
 
-  Definition f_rel (vx: int) (s: spec_state) (r: option val) (s': spec_state) :=
-    ∃ vy:int, s !! "Y" = Some (Vint32 vy) ∧
-              r = Some (Vint32 (Int.add vx vy)) ∧
-              s' = <[ "Y" := (Vint32 (Int.add vx vy)) ]> s.
+  Definition f_rel (vx: int8) (s: spec_state) (r: option val) (s': spec_state) :=
+    ∃ vy:int8, s !! "Y" = Some (Vint8 vy) ∧
+              r = Some (Vint8 (Byte.add vx vy)) ∧
+              s' = <[ "Y" := (Vint8 (Byte.add vx vy)) ]> s.
 
   Definition int_ctx := @interrupt.int_ctx _ _ invs 1 i.
 
   Lemma f_spec γ γp f vx Φ k ks:
-    f T↦ Function Tint32 [("x", Tint32)] f_body ∗
+    f T↦ Function Tint8 [("x", Tint8)] f_body ∗
     int_ctx γ γp ∗ inv N spec_inv ∗ hpri invs γp 1 ∗
     own_scode (SCrel (f_rel vx)) ∗
     (∀ v, own_scode (SCdone (Some v)) -∗ hpri invs γp 1 -∗
           WP (fill_ectxs (Evalue v) k, ks) {{ _, Φ }})
-    ⊢ WP (fill_ectxs (Ecall Tint32 f (Evalue (Vpair vx Vvoid))) k, ks) {{ _, Φ }}.
+    ⊢ WP (fill_ectxs (Ecall Tint8 f (Evalue (Vpair vx Vvoid))) k, ks) {{ _, Φ }}.
   Proof.
     iIntros "(? & #? & #? & Hp & Hsc & HΦ)".
-    iApply (wp_call _ (Vpair (Vint32 vx) Vvoid) [("x", Tint32)] f_body)=>//.
+    iApply (wp_call _ (Vpair (Vint8 vx) Vvoid) [("x", Tint8)] f_body)=>//.
     iFrame. iIntros "!>".
     wp_alloc px as "Hpx". wp_let. iApply wp_seq=>//.
     iApply cli_spec. iFrame "#". iFrame.
@@ -51,7 +51,7 @@ Section example.
     iDestruct "HI" as (vy) "[Hy HY]". iApply fupd_wp.
     (* Open invariant *)
     iInv N as ">Hspec" "Hclose".
-    iMod (spec_update {[ "Y" := Vint32 vy ]} {[ "Y" := Vint32 (Int.add vx vy) ]} with "[Hspec HY Hsc]")
+    iMod (spec_update {[ "Y" := Vint8 vy ]} {[ "Y" := Vint8 (Int.add vx vy) ]} with "[Hspec HY Hsc]")
       as "(Hspec & Hss' & Hsc' & ?)"; [ | iFrame; by iApply mapsto_singleton | ].
     { apply spec_step_rel'. unfold f_rel. eexists _. by gmap_simplify. }
     (* close invariant *)
