theories/tests/higher_order.v
@@ -5,16 +5,16 @@ Section example.
 
   Definition abs_spec g E (P Q: iProp Σ) :=
     (∃ gbody, g T↦ Function Tvoid [] gbody ∗
-                (∀ Φ k ks, P -∗ (Q -∗ WP (fill_ectxs void k, ks) {{ Φ }}) -∗
-                           WP (gbody, Kcall k::ks) @ E {{ Φ }}))%I.
+                (∀ Φ k ks Ω, P -∗ (Q -∗ WP (fill_ectxs void k, (ks, Ω)) {{ Φ }}) -∗
+                             WP (gbody, (Kcall k Ω::ks, semp)) @ E {{ Φ }}))%I.
 
-  Lemma higher_order_spec k ks E g Φ P Q:
-    abs_spec g E P Q ∗ P ∗ (Q -∗ WP (fill_ectxs void k, ks) {{ Φ }})
-    ⊢ WP (fill_ectxs (Ecall Tvoid g Vvoid) k, ks) @ E {{ Φ }}.
+  Lemma higher_order_spec k ks E g Φ P Q Ω:
+    abs_spec g E P Q ∗ P ∗ (Q -∗ WP (fill_ectxs void k, (ks, Ω)) {{ Φ }})
+    ⊢ WP (fill_ectxs (Ecall Tvoid g Vvoid) k, (ks, Ω)) @ E {{ Φ }}.
   Proof.
     iIntros "(Hg & HP & HΦ)".
     iDestruct "Hg" as (e) "[Ht He]".
-    iApply (wp_call _ Vvoid); last iFrame; first done.
+    iApply (wp_call semp Ω _ Vvoid); last iFrame; first done.
     iNext. iApply ("He" with "HP").
     iApply "HΦ".
   Qed.
