theories/clang/lib/page_table.v
@@ -1,36 +1,38 @@
-(* Virtual Memory Model *)
+(* (* Virtual Memory Model *) *)
 
-Require Import iris_c.clang.logic.
+(* Require Import iris_c.clang.lang. *)
+(* Require Import iris_c.clang.logic. *)
 
-Definition option_addr_to_val (opt_a: option addr) : val :=
-  match opt_a with
-    | Some a => Vptr a
-    | None => Vnull
-  end.
+(* Definition option_addr_to_val (opt_a: option addr) : val := *)
+(*   match opt_a with *)
+(*     | Some a => Vptr a *)
+(*     | None => Vnull *)
+(*   end. *)
 
-Structure page_table Σ `{!clangG Σ} :=  {
-  (* -- operations -- *)
-  insert_pt : ident;
-  delete_pt : ident;
-  lookup_pt : ident;
-  (* -- predicates -- *)
-  is_page_table: gmap int32 addr → iProp Σ;
-  (* -- operation specs -- *)
-  insert_pt_spec i l m Φ ks:
-    is_page_table m ∗ (is_page_table (<[ i := l ]> m) -∗ Φ Vvoid)
-    ⊢ WP (Ecall Tvoid insert_pt (Evalue (Vpair (Vint32 i) (Vpair (Vptr l) Vvoid))), ks) {{ Φ }};
-  delete_pt_spec i m Φ ks:
-    is_page_table m ∗ (is_page_table (delete i m) -∗ Φ Vvoid)
-    ⊢ WP (Ecall Tvoid delete_pt (Evalue (Vpair (Vint32 i) Vvoid)), ks) {{ Φ }};
-  lookup_pt_spec i m Φ ks:
-    is_page_table m ∗ (is_page_table m -∗ Φ (option_addr_to_val (m !! i)))
-    ⊢ WP (Ecall (Tptr Tvoid) lookup_pt (Evalue (Vpair (Vint32 i) Vvoid)), ks) {{ Φ }}
-}.
+(* Structure page_table `{clangG Σ} :=  { *)
+(*   (* -- operations -- *) *)
+(*   insert_pt : ident; *)
+(*   delete_pt : ident; *)
+(*   lookup_pt : ident; *)
+(*   (* -- predicates -- *) *)
+(*   is_page_table: gmap int8 addr → iProp Σ; *)
+(*   (* -- operation specs -- *) *)
+(*   insert_pt_spec i l m Φ ks: *)
+(*     is_page_table m ∗ (is_page_table (<[ i := l ]> m) -∗ Φ Vvoid) *)
+(*     ⊢ WP (Ecall Tvoid insert_pt *)
+(*                 (Evalue (Vpair (Vint8 i) (Vpair (Vptr l) Vvoid))), ks) {{ Φ }} *)
+(*   (* delete_pt_spec i m Φ (ks: stack * env): *) *)
+(*   (*   is_page_table m ∗ (is_page_table (delete i m) -∗ Φ Vvoid) *) *)
+(*   (*   ⊢ WP (Ecall Tvoid delete_pt (Evalue (Vpair (Vint8 i) Vvoid)), ks) {{ Φ }} *) *)
+(*   (* lookup_pt_spec i m Φ ks: *) *)
+(*   (*   is_page_table m ∗ (is_page_table m -∗ Φ (option_addr_to_val (m !! i))) *) *)
+(*   (*   ⊢ WP (Ecall (Tptr Tvoid) lookup_pt (Evalue (Vpair (Vint32 i) Vvoid)), ks) {{ Φ }} *) *)
+(* }. *)
 
-Arguments insert_pt {_ _} _.
-Arguments delete_pt {_ _} _.
-Arguments lookup_pt {_ _} _.
-Arguments insert_pt_spec {_ _} _ _ _ _ _ _.
-Arguments delete_pt_spec {_ _} _ _ _ _ _.
-Arguments lookup_pt_spec {_ _} _ _ _ _ _.
-Arguments is_page_table {_ _} _ _.
+(* Arguments insert_pt {_ _} _. *)
+(* Arguments delete_pt {_ _} _. *)
+(* Arguments lookup_pt {_ _} _. *)
+(* Arguments insert_pt_spec {_ _} _ _ _ _ _ _. *)
+(* Arguments delete_pt_spec {_ _} _ _ _ _ _. *)
+(* Arguments lookup_pt_spec {_ _} _ _ _ _ _. *)
+(* Arguments is_page_table {_ _} _ _. *)
