theories/clang/lib/refine_sound.v
@@ -31,7 +31,7 @@ Section sound.
 Lemma wp_step R e1 l1 σ1 e2 l2 σ2 efs Φ :
   (R ⊢ |==> ▷ R) →
   prim_step e1 l1 σ1 e2 l2 σ2 efs →
-  world σ1 ∗ R ∗ WP (e1, l1) {{ Φ }} ==∗ ▷ |==> ◇ (world σ2 ∗ R ∗ WP (e2, l2) {{ Φ }} ∗ wptp (map (,[]) efs)).
+  world σ1 ∗ R ∗ WP (e1, l1) {{ Φ }} ==∗ ▷ |==> ◇ (world σ2 ∗ R ∗ WP (e2, l2) {{ Φ }} ∗ wptp (map (,([], semp)) efs)).
 Proof.
   rewrite {1}wp_unfold /wp_pre.
   iIntros (HR Hstep) "[(Hw & HE & Hσ) [HR [H|[_ H]]]]".
@@ -43,7 +43,7 @@ Proof.
   iMod ("H" $! (e2, l2) σ2 efs with "[%] [$Hw $HE]") as ">($ & $ & $ & $ & ?)"=>//.
   iFrame.
   iDestruct (@big_sepL_fmap _ (expr clang_lang) (expr clang_lang * local_state clang_lang)
-                            (,[]) (fun _ x => (WP x {{ _, True }})%I) efs with "~") as "?".
+                            (,([], semp)) (fun _ x => (WP x {{ _, True }})%I) efs with "~") as "?".
   auto.
 Qed.
 
@@ -55,9 +55,9 @@ Qed.
   Proof.
     iIntros (HR Hstep) "(HW & HR & He & Ht)".
     destruct Hstep as [e1' l1' σ1' e2' l2' σ2' efs [|? t1'] t2' ?? Hstep]; simplify_eq/=.
-    - iExists (e2', l2'), (t2' ++ map (,[]) efs); iSplitR; first eauto.
+    - iExists (e2', l2'), (t2' ++ map (,([], semp)) efs); iSplitR; first eauto.
       rewrite big_sepL_app. iFrame "Ht". iApply wp_step; try iFrame; eauto.
-    - iExists p, (t1' ++ (e2', l2') :: t2' ++ map (,[]) efs); iSplitR; first eauto.
+    - iExists p, (t1' ++ (e2', l2') :: t2' ++ map (,([], semp)) efs); iSplitR; first eauto.
       rewrite !big_sepL_app !big_sepL_cons big_sepL_app.
       iDestruct "Ht" as "($ & He' & $)"; iFrame "He".
       iApply wp_step; try iFrame; eauto.
