theories/lib/int.v
@@ -5,20 +5,20 @@ Require Import iris.prelude.prelude.
 From mathcomp Require Export ssreflect.
 
 Definition op_safe op (i j: nat) : Prop :=
-    Z.to_nat (Int.intval (op (Int.repr i) (Int.repr j))) = i * j.
+    Z.to_nat (Byte.intval (op (Byte.repr i) (Byte.repr j))) = i * j.
 
-Definition mul_safe := op_safe Int.mul.
+Definition mul_safe := op_safe Byte.mul.
 
-Coercion Int.repr : Z >-> int32.
+Coercion Byte.repr : Z >-> int8.
 
 Bind Scope int_scope with int.
 Delimit Scope int_scope with int.
 
-Notation "i1 + i2" := (Int.add i1%int i2%int)
+Notation "i1 + i2" := (Byte.add i1%int i2%int)
   (at level 50, left associativity) : int_scope.
-Notation "i1 * i2" := (Int.mul i1%int i2%int)
+Notation "i1 * i2" := (Byte.mul i1%int i2%int)
   (at level 40, left associativity) : int_scope.
-Notation "i1 - i2" := (Int.sub i1%int i2%int)
+Notation "i1 - i2" := (Byte.sub i1%int i2%int)
   (at level 50, left associativity) : int_scope.
 
 Ltac rewrite_byte :=
@@ -31,16 +31,4 @@ Ltac rewrite_byte :=
     | |- context [ offset_by_byte ?off (Byte.repr ?b) ] =>
       rewrite /offset_by_byte;
         replace (Z.to_nat (Byte.intval (Byte.repr b))) with (Z.to_nat b); last done
-  end.
-
-Ltac rewrite_int :=
-  match goal with
-    | |- context [ Int.mul _ (Int.repr Z0) ] => rewrite Int.mul_zero
-    | |- context [ offset_by_int32 ?off Int.zero ] =>
-      rewrite /offset_by_int32;
-        replace (Z.to_nat (Int.intval Int.zero)) with O; last done;
-        replace (off + O) with off; last done
-    | |- context [ offset_by_int32 ?off (Int.repr ?b) ] =>
-      rewrite /offset_by_int32;
-        replace (Z.to_nat (Int.intval (Int.repr b))) with (Z.to_nat b); last done
   end.
